sub1/sub1.v
@@ -1,14 +1,22 @@
 Require Import Braun.tmonad.monad.
-Require Import Braun.common.util.
+Require Import Braun.common.util Braun.common.big_oh Braun.common.le_util.
 Require Import Arith Arith.Even Arith.Div2.
 Require Import Coq.Program.Wf.
 
-(* This file exists only to check that
-   the rkt version of sub1 really does
-   compute n-1. The running time aspects
-   of this function are complex. *)
+Require Import Coq.Program.Wf Arith.Even Arith.Div2 Arith Init.Wf.
 
-Definition sub1_result (n:nat) (res:nat) (c:nat) := n-1 = res.
+Include WfExtensionality.
+
+Program Fixpoint sub1_time (n:nat) {measure n} :=
+  match n with
+    | 0 => 3
+    | S _ => if (even_odd_dec n)
+             then (sub1_time (div2 n)) + 12
+             else 8
+  end.
+
+Definition sub1_result (n:nat) (res:nat) (c:nat) := 
+  n-1 = res /\ c = sub1_time n.
 Hint Unfold sub1_result.
 
 Load "sub1_gen.v".
@@ -16,8 +24,12 @@ Load "sub1_gen.v".
 Next Obligation.
   clear H2 am.
   rename H into EW.
-  unfold sub1_result in *.
-  subst sd2.
+  rename H1 into SR.
+
+  destruct SR; subst sd2 an.
+
+  split.
+
   rewrite (even_double (S wildcard')) at 1; auto.
   unfold double.
   remember (div2 (S wildcard')) as x.
@@ -28,4 +40,80 @@ Next Obligation.
   inversion H0.
   simpl in Heqx.
   inversion Heqx.
+
+  unfold_sub sub1_time (sub1_time (S wildcard')).
+  fold_sub sub1_time.
+  dispatch_if EW' EW''; intuition.
+  assert False; intuition.
+  apply (not_even_and_odd (S wildcard')); auto.
 Qed.
+
+Next Obligation.
+  split;auto.
+  unfold_sub sub1_time (sub1_time (S wildcard')).
+  fold_sub sub1_time.
+  dispatch_if EW EW'; intuition.
+  assert False; intuition.
+  apply (not_even_and_odd (S wildcard')); auto.
+Qed.
+
+Fixpoint sub1_linear_time n :=
+  match n with
+    | 0 => 3
+    | S n' => sub1_time n + sub1_linear_time n' + 7
+  end.
+
+Definition sub1_linear_loop_result (n:nat) (res:nat) (c:nat) :=
+  c = sub1_linear_time n.
+Hint Unfold sub1_linear_loop_result.
+
+Load "sub1_linear_loop_gen.v".
+
+Next Obligation.
+  rename H into SUB1R.
+  destruct SUB1R.
+  omega.
+Qed.
+
+Next Obligation.
+  clear H2 am0 am H3 sub1_linear_loop.
+  rename H1 into SUB1_RESULT.
+  
+  unfold sub1_linear_loop_result in *.
+  destruct SUB1_RESULT.
+  subst an an0 n'.
+  unfold sub1_linear_time; fold sub1_linear_time.
+  replace (S wildcard' - 1) with wildcard'; omega.
+Qed.
+
+Program Fixpoint sub1_time2 (n:nat) {measure n} :=
+  match n with
+    | 0 => 0
+    | S _ => if (even_odd_dec n)
+             then (sub1_time2 (div2 n)) + 1
+             else 1
+  end.
+
+Lemma sub1_time12 : big_oh sub1_time sub1_time2.
+  exists 1.
+  exists 50.
+  intros n LE.
+  destruct n; intuition.
+  clear LE.
+  apply (well_founded_induction
+           lt_wf
+           (fun n => sub1_time (S n) <= 50 * sub1_time2 (S n))).
+  clear n; intros n IND.
+  unfold_sub sub1_time (sub1_time (S n)); fold_sub sub1_time.
+  unfold_sub sub1_time2 (sub1_time2 (S n)); fold sub1_time2.
+  dispatch_if COND1 COND1'; try omega.
+  destruct n.
+  simpl; omega.
+  rewrite mult_plus_distr_l.
+  replace (50*1) with (38+12); [|omega].
+  rewrite plus_assoc.
+  apply le_plus_left.
+  apply le_add_right.
+  apply IND; auto.
+Qed.
+
